

$$\begin{aligned}
 1. \quad \Pr(X=Y) &= \sum_{t \in \Omega} \Pr(X=Y=t) \\
 &\leq \sum_{t \in \Omega} \min\{\Pr(X=t), \Pr(Y=t)\} \\
 &= \sum_{t \in \Omega} \min\{\mu(t), \nu(t)\}.
 \end{aligned}$$

Thus,

$$\begin{aligned}
 \Pr(X \neq Y) &= 1 - \Pr(X=Y) \\
 &\geq 1 - \sum_{t \in \Omega} \min\{\mu(t), \nu(t)\} \\
 &= \sum_{t \in \Omega} \mu(t) - \sum_{t \in \Omega} \min\{\mu(t), \nu(t)\} \\
 &= \sum_{t \in \Omega} (\mu(t) - \min\{\mu(t), \nu(t)\}) \\
 &= \sum_{\substack{t \in \Omega \\ \mu(t) > \nu(t)}} (\mu(t) - \nu(t)) \\
 &= \max_{A \subseteq \Omega} |\mu(A) - \nu(A)| \\
 &= D_{TV}(\mu, \nu).
 \end{aligned}$$

If  $\Pr(X \neq Y) = D_{TV}(\mu, \nu)$ , we have

$$\Pr(X=Y=t) = \min\{\mu(t), \nu(t)\}.$$

Give an explicit construction of  $\omega$  below:

$$\omega_{i,j} = \begin{cases} \min\{\mu(i), \nu(i)\}, & i=j \\ k \max\{0, \nu(i) - \mu(i)\} \max\{0, \mu(j) - \nu(j)\}, & i \neq j, \end{cases} \quad k \text{ is a constant.}$$

First, if there exist  $k \in \mathbb{R}$  such that  $\omega$  is a coupling,  $\Pr_{(X,Y) \sim \omega}(X \neq Y) = D_{TV}(\mu, \nu)$ .

Then, compute  $k$ .

$$\begin{cases} \sum_j \omega_{ij} = \mu(i) & \forall i \in [|\Omega|] \\ \sum_i \omega_{ij} = \nu(j) & \forall j \in [|\Omega|] \end{cases}$$

Consider one of these equations.

$$\begin{aligned}
 \mu(i) &= \sum_j \omega_{ij} = \sum_{j \neq i} k \max\{0, \nu(i) - \mu(i)\} \max\{0, \mu(j) - \nu(j)\} + \min\{\mu(i), \nu(i)\} \\
 &= k \max\{0, \nu(i) - \mu(i)\} (D_{TV}(\mu, \nu) - \max\{0, \mu(j) - \nu(j)\}) + \min\{\mu(i), \nu(i)\}.
 \end{aligned}$$

If  $\nu(i) - \mu(i) > 0$

$$\begin{aligned}
 \mu(i) &= k(\nu(i) - \mu(i)) D_{TV}(\mu, \nu) + \mu(i) \\
 \Rightarrow k &= \frac{1}{D_{TV}(\mu, \nu)}
 \end{aligned}$$

If  $\nu(i) - \mu(i) \leq 0$

$$\mu(i) = \nu(i) \quad \checkmark.$$

So  $k = \frac{1}{D_{TV}(\mu, \nu)}$  is a solution to

all  $2|\Omega|$  equations.

$$\text{Thus, } \omega_{i,j} = \begin{cases} \min\{\mu(i), \nu(i)\}, & i=j \\ \frac{1}{D_{TV}(\mu, \nu)} \max\{0, \nu(i) - \mu(i)\} \max\{0, \mu(j) - \nu(j)\}, & i \neq j \end{cases}$$

is a distribution that meets the conditions.



Not use coupling:

$$2. \quad \begin{cases} \textcircled{1} \mu_t^T = \mu_0^T P^t \\ \mu_{t+1}^T = \mu_0^T P^{t+1} \end{cases} \Rightarrow \mu_{t+1}^T = \mu_t^T P$$

For a transition matrix  $P$ ,

$$\begin{cases} \sum_j P_{ij} = 1 \quad \sum_i P_{ij} = 1 \quad \forall i, j \\ \forall i, j, P_{ij} \geq 0 \end{cases}$$

$$\pi^T = \pi^T P$$

$$\textcircled{2} \text{ For a vector } X = (x_1, x_2, \dots, x_n), \|X\|_F \triangleq \sum_{i=1}^n |x_i|.$$

$$\Delta(t) = D_{TV}(\mu_t, \pi) = \frac{1}{2} \sum_{i=1}^{|N|} |\mu_t(i) - \pi(i)| = \frac{1}{2} \|\mu_t - \pi\|_F.$$

$$\begin{aligned} \text{Similarly, } \Delta(t+1) &= \frac{1}{2} \|\mu_{t+1} - \pi\|_F = \frac{1}{2} \|P^T \mu_t - \pi\|_F \\ &= \frac{1}{2} \|P^T \mu_t - P^T \pi\|_F = \frac{1}{2} \|P^T (\mu_t - \pi)\|_F \end{aligned}$$

$$\textcircled{3} X_t \triangleq \mu_t - \pi, \quad \sum_i X_{ti} = \sum_i \mu_t(i) - \sum_i \pi(i) = 1 - 1 = 0$$

$$\text{Thus, } \Delta(t) = \frac{1}{2} \|X_t\|_F = \frac{1}{2} \sum_{i=1}^{|N|} |X_{ti}|$$

$$\begin{aligned} \Delta(t+1) &= \frac{1}{2} \|P^T X_t\|_F = \frac{1}{2} \sum_{i=1}^{|N|} |P_{1i} X_{t1} + P_{2i} X_{t2} + \dots + P_{|N|i} X_{t|N|}| \\ &\leq \frac{1}{2} \sum_{i=1}^{|N|} (P_{1i} |X_{t1}| + \dots + P_{|N|i} |X_{t|N|}|) \\ &= \frac{1}{2} \sum_{i=1}^{|N|} \left( \left( \sum_{j=1}^{|N|} P_{ji} \right) |X_{ti}| \right) \\ &= \frac{1}{2} \sum_{i=1}^{|N|} |X_{ti}| = \Delta(t) \end{aligned}$$

Use coupling:

Assume  $X_t \sim \mu_t$ ,  $Y_t \sim \pi$ ,  $\omega$  is a coupling of  $X_t$  and  $Y_t$ .

Then  $\Delta(t) = D_{TV}(\mu_t, \pi) \leq \Pr_{(X_t, Y_t) \sim \omega}(X_t \neq Y_t)$ .  
Similarly,  $\Delta(t+1) \leq \Pr(X_{t+1} \neq Y_{t+1})$ , if  $X_{t+1} \sim \mu_{t+1}$ ,  $Y_{t+1} \sim \pi$ .  
And in fact as what we have proved in Problem 1.

there exist an  $\omega$  such that  $\Delta(t) = \Pr_{(X_t, Y_t) \sim \omega}(X_t \neq Y_t)$ .

Consider this  $\omega$ . Let  $\omega'$  be a coupling such that:

- ①  $\omega'$  is a coupling of  $X_{t+1}$  and  $Y_{t+1}$ ;
- ② If  $X_t = Y_t$ , then  $X_{t+1}$  and  $Y_{t+1}$  are evolved from  $X_t$  and  $Y_t$  synchronously.  
which assures that if  $X_t = Y_t$ ,  $X_{t+1} = Y_{t+1}$ ;
- ③ If  $X_t \neq Y_t$ , then  $X_{t+1}$  and  $Y_{t+1}$  are evolved from  $X_t$  and  $Y_t$  respectively.

With ①②③, we have  $\Pr(X_t = Y_t) \leq \Pr(X_{t+1} = Y_{t+1})$ ,

$$\Leftrightarrow \Pr(X_t \neq Y_t) \geq \Pr(X_{t+1} \neq Y_{t+1}).$$

Then  $\Delta(t) = \Pr(X_t \neq Y_t) \geq \Pr(X_{t+1} \neq Y_{t+1}) \geq \Delta(t+1)$ .



$$3. \quad E(HH) = 1 + \frac{1}{2}E(HH|H) + \frac{1}{2}E(HH|T)$$

$$E(HH|H) = \frac{1}{2} \times 1 + \frac{1}{2} \times (1 + E(HH|HT))$$

$$= \frac{1}{2} \times 1 + \frac{1}{2} \times (1 + E(HH|T))$$

$$= 1 + \frac{1}{2}E(HH|T)$$

$$E(HH|T) = \frac{1}{2}(1 + E(HH|HT)) + \frac{1}{2}(1 + E(HH|TT))$$

$$= \frac{1}{2} \left( 2 + \frac{1}{2}E(HH|T) \right) + \frac{1}{2}(1 + E(HH|T))$$

$$= \frac{3}{2} + \frac{3}{4}E(HH|T)$$

$$\Rightarrow E(HH|T) = 6$$

$$\Rightarrow E(HH|H) = 4$$

$$\Rightarrow E(HH) = 6$$

$$E(HT) = 1 + \frac{1}{2}E(HT|H) + \frac{1}{2}E(HT|T)$$

$$E(HT|H) = \frac{1}{2} \times (1 + E(HT|HT)) + \frac{1}{2} \times 1$$

$$\Rightarrow E(HT|H) = 2$$

$$E(HT|T) = \frac{1}{2} \times (1 + E(HT|HT)) + \frac{1}{2} \times (1 + E(HT|TT))$$

$$= 2 + \frac{1}{2}E(HT|T)$$

$$\Rightarrow E(HT|T) = 4$$

$$\Rightarrow E(HT) = 4$$

$$\text{So } E(T_1) = 6, E(T_2) = 4$$

We can say that HT will be seen faster from the probability point of view.

(1) Firstly, consider the case when  $k=2$ .

$$\begin{aligned}
 \Pr(z_2''=c) &= \sum_{z_1''} \Pr(z_1'=a) \Pr(z_2''=c | z_1'=a) \\
 (z_0', z_1') \in \omega_1 & \\
 z_1' &= z_1'' \\
 (z_1', z_2'') \in \omega_2 & \\
 &= \sum_{z_1'} \Pr(z_1'=a) \Pr(z_2''=c | z_1'=a) \\
 &= \sum_{z_1'} \left( \sum_{z_0'} \Pr(z_0'=b) \Pr(z_1'=a | z_0'=b) \right) \Pr(z_2''=c | z_1'=a) \\
 &\stackrel{\text{fix } z_0'}{=} \sum_{z_0'} \Pr(z_0'=b) \left( \sum_{z_1'} \Pr(z_1'=a | z_0'=b) \Pr(z_2''=c | z_1'=a, z_0'=b) \right) \\
 &= \sum_{z_0'} \Pr(z_0'=b) \left( \sum_{z_1'} \frac{\Pr(z_1'=a, z_0'=b)}{\Pr(z_0'=b)} \frac{\Pr(z_1'=a, z_0'=b, z_2''=c)}{\Pr(z_1'=a, z_0'=b)} \right) \\
 &= \sum_{z_0'} \Pr(z_0'=b) \sum_{z_1'} \Pr(z_1'=a, z_2''=c | z_0'=b) \\
 &= \sum_{z_0'} \Pr(z_0'=b) \Pr(z_2''=c | z_0'=b) \\
 &= \Pr(z_2''=c), \text{ i.e. } (z_0, z_2) \text{ is a legal coupling of } (X_t, Y_t). \\
 (z_0', z_2'') &\in \omega
 \end{aligned}$$

For all  $k \in \mathbb{N}^+$ , we can prove similarly that if  $(z_0, z_{k-1})$  is a legal coupling,  $(z_0, z_k)$  is a legal coupling.

By induction,  $(z_0, z_k)$  is a legal coupling of  $(X_t, Y_t)$  for all  $k \in \mathbb{N}^+$ .

(2) For  $d(X_t, Y_t)=1$ ,  $\mathbb{E}(d(X_{t+1}, Y_{t+1}) | (X_t, Y_t)) \leq (1-\alpha) d(X_t, Y_t)$

Compute expectations on both sides.

$$\mathbb{E}(\mathbb{E}(d(X_{t+1}, Y_{t+1}) | (X_t, Y_t))) \leq (1-\alpha) \mathbb{E}(d(X_t, Y_t))$$

$$\Rightarrow \mathbb{E}(d(X_{t+1}, Y_{t+1})) \leq 1-\alpha \text{ for those } d(X_t, Y_t)=1.$$

For  $d(z_i, z_{i+1})=1$  for  $i=0, 1, \dots, k-1$ ,  $\mathbb{E}(d(z_i, z_{i+1})) \leq 1-\alpha$

$$d(z_0, z_k) \leq d(z_0, z_1) + d(z_1, z_2) + \dots + d(z_{k-1}, z_k)$$

Compute expectations on both sides.

$$\mathbb{E}(d(z_0, z_k)) \leq \mathbb{E}(d(z_0, z_1) + d(z_1, z_2) + \dots + d(z_{k-1}, z_k)) = \sum_{i=0}^{k-1} \mathbb{E}(d(z_i, z_{i+1})) \leq (1-\alpha)k.$$



(3) Consider the probabilities of two types of moves.

For good moves, w.p.  $\frac{d(X_t, Y_t)}{n}$ ,  $X_t(v) \neq Y_t(v)$ , and all choices of color  $c$  can make it a good move, since we have added these improper colorings to  $\Omega$ .

$$\Pr(d(X_{t+1}, Y_{t+1}) = d(X_t, Y_t) - 1) = \Pr((v, c) \text{ is a good move}) \geq \frac{d(X_t, Y_t)}{n}$$

For bad moves, there exists a neighbor  $w$  of  $v$  that its color is different in two colorings, and in one coloring  $w$  is of color  $c$ .

$$\Pr(d(X_{t+1}, Y_{t+1}) = d(X_t, Y_t) + 1) = \Pr((v, c) \text{ is a bad move}) \leq \frac{\Delta d(X_t, Y_t)}{n} \frac{2}{q}$$

$$\begin{aligned} \mathbb{E}(d(X_{t+1}, Y_{t+1}) | (X_t, Y_t)) &= d(X_t, Y_t) + \Pr(d(X_{t+1}, Y_{t+1}) = d(X_t, Y_t) + 1) - \Pr(d(X_{t+1}, Y_{t+1}) = d(X_t, Y_t) - 1) \\ &\leq d(X_t, Y_t) \left(1 + \frac{2\Delta}{nq} - \frac{1}{n}\right) = d(X_t, Y_t) \left(1 - \frac{q-2\Delta}{nq}\right) \end{aligned}$$

$$\text{In the case } q > 2\Delta, \quad \mathbb{E}(d(X_{t+1}, Y_{t+1}) | (X_t, Y_t)) \leq d(X_t, Y_t) \left(1 - \frac{1}{nq}\right)$$

$$\text{If we want } D_{TV} \leq \left(1 - \frac{1}{nq}\right)^t h \leq \varepsilon.$$

$$\text{we have } \tau_{\text{mix}}(\varepsilon) \leq nq \log \frac{n}{\varepsilon} = O(n \log n)$$